content/src/html.rs
@@ -1,3 +1,9 @@
 mod environment_settings_object;
+mod html_anchor_element;
+mod html_element;
+mod html_parser;
 
 pub use environment_settings_object::EnvironmentSettingsObject;
+pub use html_anchor_element::HTMLAnchorElement;
+pub use html_element::HTMLElement;
+pub use html_parser::{JsHtmlParserProvider, execute_parser_scripts, parse_html_into_document};
